src/RIoT.Stubs.fst
@@ -26,3 +26,27 @@ module B   = LowStar.Buffer
 module M   = LowStar.Modifies
 module HS  = FStar.HyperStack
 module HST = FStar.HyperStack.ST
+
+assume val riotCrypt_Hash
+  (size: I.uint_32)
+  (data: B.lbuffer uint8 (v size))
+  (digest_alg: hash_alg)
+  (digest: hash_t digest_alg)
+: HST.Stack unit
+  (requires fun h ->
+      B.live h data
+    /\ B.live h digest
+    /\ B.disjoint data digest)
+  (ensures  fun h0 _ h1 ->
+      B.modifies (B.loc_buffer digest) h0 h1)
+
+assume val riotCrypt_DeriveEccKey
+  (public_key : riot_ecc_publickey)
+  (private_key: riot_ecc_privatekey)
+  (digest_alg: hash_alg)
+  (digest: hash_t digest_alg)
+  (label_size: I.uint_32)
+  (label: B.lbuffer uint8 (I.v label_size))
+: HST.Stack unit
+  (requires fun h -> True)
+  (ensures  fun h0 _ h1 -> True)
