src/RIoT.X509.fst
@@ -1,0 +1,124 @@
+module RIoT.X509
+
+open Common
+
+open LowStar.BufferOps
+open Lib.IntTypes
+
+open Spec.Hash.Definitions
+open Hacl.Hash.Definitions
+
+module I  = FStar.Integers
+module HI  = Lib.IntTypes
+
+module SHA2= Hacl.Hash.SHA2
+module HMAC= Hacl.HMAC
+module Ed25519 = Hacl.Ed25519
+
+module CL  = C.Loops
+module CE  = C.Endianness
+module CF  = C.Failure
+module C   = C
+module CS  = C.String
+module S   = FStar.Seq
+module IB  = LowStar.ImmutableBuffer
+module B   = LowStar.Buffer
+module M   = LowStar.Modifies
+module HS  = FStar.HyperStack
+module HST = FStar.HyperStack.ST
+
+let _BIGLEN : I.uint_32 = 0x09ul
+
+noeq
+type bigval_t = {
+     data : B.lbuffer uint32 (v _BIGLEN)
+  }
+
+/// REF:
+/// typedef struct {
+///     bigval_t x;
+///     bigval_t y;
+///     uint32_t infinity;
+/// } affine_point_t;
+noeq
+type affine_point_t = {
+     x: bigval_t;
+     y: bigval_t;
+     infinity: B.pointer uint32
+  }
+type riot_ecc_publickey = affine_point_t
+
+
+let live_affine_point
+  (h: HS.mem)
+  (p: affine_point_t)
+: Type0
+=   B.live h p.x.data
+  /\ B.live h p.y.data
+  /\ B.live h p.infinity
+let live_ecc_publickey = live_affine_point
+
+/// REF:
+/// typedef struct {
+///     bigval_t r;
+///     bigval_t s;
+/// } ECDSA_sig_t;
+noeq
+type ecdsa_sig_t = {
+     r: bigval_t;
+     s: bigval_t
+  }
+type riot_ecc_privatekey = ecdsa_sig_t
+
+let live_ecdsa_sig
+  (h: HS.mem)
+  (s: ecdsa_sig_t)
+: Type0
+=   B.live h s.r.data
+  /\ B.live h s.s.data
+type live_ecc_privatekey = live_ecdsa_sig
+
+
+let riot_kdf_fixed
+  (fixed_size: I.uint_32{(v fixed_size) > 0})
+  (fixed: B.lbuffer uint8 (v fixed_size))
+  (label_size: I.uint_32)
+  (label: B.lbuffer uint8 (v label_size))
+  (context_size: I.uint_32)
+  (context: B.lbuffer uint8 (v context_size))
+  (numberOfBits: I.uint_32)
+: HST.Stack unit
+  (requires fun h ->
+      B.live h fixed
+    /\ B.live h label
+    /\ B.live h context
+    /\ B.disjoint fixed label
+    /\ B.disjoint fixed context
+    /\ B.disjoint context label)
+  (ensures  fun h0 _ h1 -> True)
+=
+  HST.push_frame();
+
+  let total_size: I.uint_32 =
+      (if (!*fixed) = (u8 0x00) then fixed_size else 0ul)
+    + (if (!*label) = (u8 0x00) then label_size else 0ul) in
+
+  HST.pop_frame()
+
+let ecdh_derive
+  (p1: affine_point_t)
+  (k: bigval_t)
+  (src: bigval_t)
+  (label_size: I.uint_32)
+  (label: B.lbuffer uint8 (I.v label_size))
+: HST.Stack unit
+  (requires fun h ->
+      live_affine_point h p1
+    /\ B.live h k.data)
+  (ensures  fun h0 _ h1 -> True)
+=
+  HST.push_frame();
+
+  k.data.(1ul) <- (u32 0);
+
+  HST.pop_frame()
